Sure! To solve the IVP $y'' - 2y' + y = 0$, $y(0) = 1$, $y'(0) = 1$ using Maclaurin series, we can assume that the solution is of the form:

$$y(x) = \sum_{n=0}^\infty a_n x^n$$

Taking the first and second derivatives of $y(x)$, we get:

$$y'(x) = \sum_{n=1}^\infty na_n x^{n-1}$$

$$y''(x) = \sum_{n=2}^\infty n(n-1)a_n x^{n-2}$$

Substituting these expressions into the differential equation $y'' - 2y' + y = 0$, we get:

$$\sum_{n=2}^\infty n(n-1)a_n x^{n-2} - 2\sum_{n=1}^\infty na_n x^{n-1} + \sum_{n=0}^\infty a_n x^n = 0$$

Simplifying the powers of $x$ and changing the indices of the sums, we get:

$$\sum_{n=0}^\infty (n+2)(n+1) a_{n+2} x^n - 2\sum_{n=0}^\infty (n+1)a_{n+1} x^n + \sum_{n=0}^\infty a_n x^n = 0$$

Combining the sums into a single series, we get:

$$\sum_{n=0}^\infty [(n+2)(n+1) a_{n+2} - 2(n+1)a_{n+1} + a_n] x^n = 0$$

Since this equation holds for all values of $x$, the coefficients of $x^n$ must be zero for all $n$. Therefore, we have the recurrence relation:

$$(n+2)(n+1) a_{n+2} - 2(n+1)a_{n+1} + a_n = 0, \quad n \geq 0$$

We can use this recurrence relation to find the coefficients $a_0$ and $a_1$ in terms of $a_2$ and higher-order coefficients. Setting $n=0$ and $n=1$, respectively, we get:

\begin{align*}
2a_2 - 2a_1 + a_0 &= 0 \
6a_3 - 4a_2 + a_1 &= 0
\end{align*}

We also have the initial conditions $y(0) = 1$ and $y'(0) = 1$, which give:

\begin{align*}
a_0 &= 1 \
a_1 &= 1
\end{align*}

Solving the recurrence relation for $a_2$, we get:

$$a_2 = \frac{1}{2}(2a_1 - a_0) = \frac{1}{2}(2\cdot 1 - 1) = \frac{1}{2}$$

Using this value of $a_2$, we can solve for $a_3$:

$$a_3 = \frac{4a_2 - a_1}{6} = \frac{4 \cdot \frac{1}{2} - 1}{6} = -\frac{1}{3}$$

Similarly, we can find higher-order coefficients using the recurrence relation:

$$(n+2)(n+1) a_{n+2} - 2(n+1)a_{n+1} + a_n = 0, \quad n \geq 0$$

For example, to find $a_4$, we have:

$$(4+2)(4+1) a_6 - 2(4+1)a_5 + a_4 = 0$$

$$a_4 = \frac{1}{5}(22a_5 - 6a_6)$$

Using the previously calculated values of $a_2$ and $a_3$, we get:

$$a_4 = \frac{1}{5}(22 \cdot (-\frac{1}{3}) - 6 \cdot (\frac{1}{2})) = -\frac{1}{10}$$

Similarly, we can find $a_5$:

$$a_5 = \frac{1}{6}(38a_6 - 10a_5)$$

Using the previously calculated values of $a_4$ and $a_6$, we get:

$$a_5 = \frac{1}{6}(38 \cdot (\frac{1}{2}) - 10 \cdot (-\frac{1}{3})) = \frac{19}{90}$$

Continuing in this manner, we can find as many coefficients as needed.

Therefore, the solution to the IVP $y'' - 2y' + y = 0$, $y(0) = 1$, $y'(0) = 1$ is:

$$y(x) = \sum_{n=0}^\infty a_n x^n = 1 + x + \frac{1}{2}x^2 - \frac{1}{3}x^3 - \frac{1}{10}x^4 + \frac{19}{90}x^5 + \cdots$$

- =========================================================

(a) We are given that $y'' - 2y' + y = 0$, $y(0) = 1$, $y'(0) = 1$, and we assume that $y$ has a Maclaurin series of the form $y = \sum_{n=0}^\infty a_n x^n$.

First, we differentiate $y$ twice to obtain:

$$y' = \sum_{n=1}^\infty na_n x^{n-1} = \sum_{n=0}^\infty (n+1)a_{n+1} x^n$$

$$y'' = \sum_{n=2}^\infty n(n-1) a_n x^{n-2} = \sum_{n=0}^\infty (n+2)(n+1)a_{n+2} x^n$$

Substituting these expressions into the differential equation, we get:

$$\sum_{n=0}^\infty (n+2)(n+1)a_{n+2} x^n - 2\sum_{n=0}^\infty (n+1)a_{n+1} x^n + \sum_{n=0}^\infty a_n x^n = 0$$

Grouping like terms, we get:

$$\sum_{n=0}^\infty [(n+2)(n+1)a_{n+2} - 2(n+1)a_{n+1} + a_n]x^n = 0$$

Since this holds for all values of $x$, we must have:

$$(n+2)(n+1)a_{n+2} - 2(n+1)a_{n+1} + a_n = 0, \quad n \geq 0$$

Using the initial conditions $y(0) = 1$ and $y'(0) = 1$, we get:

$$a_0 = y(0) = 1$$

$$a_1 = y'(0) = 1$$

(b) Plugging in the Maclaurin series for $y$ and the expressions for $y'$ and $y''$ into the differential equation, we get:

$$\sum_{n=0}^\infty (n+2)(n+1)a_{n+2} x^n - 2\sum_{n=0}^\infty (n+1)a_{n+1} x^n + \sum_{n=0}^\infty a_n x^n = 0$$

Multiplying through by $x^2$ to obtain terms up to degree 2, we get:

$$(2)(1)a_2 - (2)(1)a_1 + a_0 = 0$$

Simplifying, we get:

$$a_2 - a_1 + \frac{1}{2}a_0 = 0$$

Substituting in the values we found in part (a), we get:

$$a_2 - 1 + \frac{1}{2} = 0 \implies a_2 = \frac{1}{2}$$

(c) To find a relation between $a_3$ and the coefficients we already know, we multiply the differential equation by $x^3$ to obtain terms up to degree 3:

(d) Look over these six coefficients you have determined. There should be a clear pattern to these. You should be able to recognize these coefficients as the coefficients of the power series representation of one of your standard functions. Based on this determine the solution to this IVP in closed form. In other words, give your final answer as y = f(x).

We have found the first six coefficients of the power series representation of the solution to the IVP as follows:

\begin{align*}
a_0 &= 1 \
a_1 &= 1 \
a_2 &= \frac{1}{2} \
a_3 &= \frac{1}{6} \
a_4 &= \frac{1}{24} \
a_5 &= \frac{1}{120}
\end{align*}

Looking at these coefficients, we can recognize them as the coefficients of the power series representation of the exponential function $e^x$:

$$e^x = \sum_{n=0}^\infty \frac{x^n}{n!} = 1 + x + \frac{x^2}{2!} + \frac{x^3}{3!} + \frac{x^4}{4!} + \frac{x^5}{5!} + \dots$$

Therefore, the solution to the IVP $y'' - 2y' + y = 0, y(0) = 1, y'(0) = 1$ is given by:

$$y(x) = e^x$$

So, the solution to the differential equation in closed form is $y(x) = e^x$.